{
 "cells": [
  {
   "cell_type": "markdown",
   "id": "25bd0723-bec6-4a00-a16f-68a1fc66e333",
   "metadata": {},
   "source": [
    "### 2.21\n",
    "\n",
    "\n",
    "\n",
    "$\\begin{align}\\dots\\end{align}$\n",
    "\n",
    "\n",
    "\n",
    "### 2.22\n",
    "\n",
    "\n",
    "\n",
    "$\\begin{align}\\dots\\end{align}$\n",
    "\n",
    "\n",
    "\n",
    "### 2.23 Prove or counterexample: For $f$ a multiplicative function: $F$ defined below is multiplicative as well.\n",
    "\n",
    "\n",
    "$\\begin{align}F(n) = \\prod_{d|n} f(d)\\end{align}$\n",
    "\n",
    "False by counterexample: For $f(n)$ use $\\mu(30)$\n",
    "\n",
    "\n",
    "$\\begin{align}\n",
    "F_{\\mu}(30) = \\mu(1) \\cdot \\mu(2) \\cdot \\cdots \\cdot \\mu(30) = 1 \\cdot -1 \\cdot -1 \\cdot -1 \\cdot 1 \\cdot 1 \\cdot 1 \\cdot -1 = 1\n",
    "\\end{align}$\n",
    "\n",
    "\n",
    "$\\begin{align}\n",
    "F_{\\mu}(2) \\cdot F_{\\mu}(15) = (1 \\cdot -1) \\cdot (1 \\cdot -1 \\cdot -1 \\cdot 1 ) = -1\n",
    "\\end{align}$\n",
    "\n",
    "### 2.24\n",
    "\n",
    "\n",
    "$\\begin{align}\\dots\\end{align}$\n",
    "\n",
    "### 2.25 Dirichlet inverse of a multiplicative function\n",
    "\n",
    "#### 2.25 (a) For multiplicative $f$ show the Dirichlet inverse $f^{-1} = \\mu f$ for all square-free $n$.\n",
    "\n",
    "\n",
    "A Dirichlet inverse supposes functions $f$ and $f^{-1}$ with Dirichlet \n",
    "product $I(n)$. \n",
    "$f$ being multiplicative has a Dirchlet inverse for any $n \\ge 1$; but this \n",
    "problem considers only square-free values of $n$. For this subset \n",
    "$\\{ 1, 2, 3, 5, 6, 7, 10, 11, 13, 14, 15, \\dots \\}: \\; f$ is\n",
    "*de facto* completely multiplicative: The decomposition of a square-free \n",
    "argument into products $n = a_1 \\cdot a_2 \\cdots a_q$ will necessarily\n",
    "have $(a_i, a_j) = 1$. Consequently the inverse of $f$ is $\\mu f$\n",
    "over square-free $n$.\n",
    "\n",
    "\n",
    "The above as a solution is dubious. Here is a more extensive run at the task:\n",
    "\n",
    "\n",
    "A multiplicative function is not identically zero and $f(mn) = f(m) \\cdot f(n)$\n",
    "when $(m, n) = 1$. The totient $\\varphi$ is an example that is not completely\n",
    "multiplicative. The table below shows how a putative inverse $\\mu \\varphi$ works \n",
    "correctly on square-free numbers: $\\varphi * (\\mu \\varphi)(n) = I(n)$.\n",
    "\n",
    "\n",
    "<table style=\"margin-left: 0;\">\n",
    "<tr><th>n</th><th>$\\varphi$</th><th>$\\mu$</th><th>$\\mu \\varphi$</th><th>$\\varphi * (\\mu \\varphi)$</th></tr>\n",
    "<tr><td>1</td><td>1</td><td>1</td><td>1</td><td>1</td>\n",
    "<tr><td>2</td><td>1</td><td>-1</td><td>-1</td><td>0</td>\n",
    "<tr><td>3</td><td>2</td><td>-1</td><td>-2</td><td>0</td>\n",
    "<tr><td>4</td><td>2</td><td>0</td><td>0</td><td>1*</td>\n",
    "<tr><td>5</td><td>4</td><td>-1</td><td>-4</td><td>0</td>\n",
    "<tr><td>6</td><td>2</td><td>1</td><td>2</td><td>0</td>\n",
    "<tr><td>7</td><td>6</td><td>-1</td><td>-6</td><td>0</td>\n",
    "<tr><td>8</td><td>4</td><td>0</td><td>0</td><td>2*</td>\n",
    "<tr><td>9</td><td>6</td><td>0</td><td>0</td><td>2*</td>\n",
    "<tr><td>10</td><td>4</td><td>1</td><td>4</td><td>0</td>\n",
    "<tr><td>11</td><td>10</td><td>-1</td><td>-10</td><td>0</td>\n",
    "<tr><td>12</td><td>4</td><td>0</td><td>0</td><td>0*</td>\n",
    "<tr><td>13</td><td>12</td><td>-1</td><td>-12</td><td>0</td>\n",
    "<tr><td>14</td><td>6</td><td>1</td><td>6</td><td>0</td>\n",
    "</table>\n",
    "\n",
    "\n",
    "(\\* not square-free)\n",
    "\n",
    "\n",
    "Returning to $f$: For $n=1$ we have the putative inverse $(\\mu f)(1) = 1$ as necessary\n",
    "per Thm 2.8. Now for $n > 1$ with $n$ square-free, thinking about the $f * (\\mu f)$ convolution: \n",
    "Pairs of divisors of $n$ of the form $\\{ d, \\frac{n}{d} \\}$ will have $(d, n/d)=1$ as otherwise \n",
    "$n$ would not be square-free.\n",
    "As $f$ is multiplicative we have $f(d) \\cdot f(n/d) = f(d \\cdot \\frac{n}{d}) = f(n)$. \n",
    "\n",
    "\n",
    "$\\begin{align}\n",
    "(\\mu f) * f)(n) = \\sum_{d|n} \\mu(d) \\cdot f(d) \\cdot f(\\frac{n}{d}) = \n",
    "f(n)\\sum_{d|n} \\mu(d) = f(n) \\cdot I(n) = I(n).\n",
    "\\;\\;\\end{align}$\n",
    "\n",
    "\n",
    "&#x2610;\n",
    "\n",
    "\n",
    "***In passing:*** The divisors of $n>1$ can be generated as a sum from $(1 + p_1)\\cdot(1 + p_2) \\dots (1 + p_i)$. \n",
    "\n",
    "\n",
    "$\n",
    "\\begin{align}\n",
    "\\sum_{d|n} \\mu(d) = \\mu(1) + \\binom{i}{1} \\cdot \\mu(p_1) + \\binom{i}{2} \\cdot \\mu(p_1\\cdot p_2) + \\dots + \n",
    "\\mu(p_1 \\cdot p_2 \\dots p_i) = \\sum_{k=0}^{i} {-1}^k \\binom{i}{k} = 0.\n",
    "\\end{align}\n",
    "$\n",
    "\n",
    "\n",
    "(See the comment preceding problem 2.5.)\n",
    "\n",
    "##### 2.25 (b) For $f$ multiplicative: Show for any prime $p$ that $f^{-1}(p^2)=f(p)^2-f(p^2)$ \n",
    "\n",
    "\n",
    "$n = p^2$ applies to $\\{ 4, 9, 25, 49, \\dots\\}$. \n",
    "$f(1)=1$ and $f^{-1}(1)=1$. Take $n=p^2$ and $f(p^2)$ convolved with $f(p^2)-f(p)^2$ yields $0$.\n",
    "\n",
    "\n",
    "$\\begin{align}\n",
    "(f(p^2) - f(p)^2) * f(p^2) = \\; & \\sum_{d\\in\\{1,p,p^2\\}}(f(d^2)-f(d)^2)\\cdot f(\\frac{n}{d}) \\\\\n",
    "= \\; & \\bigl( f(1)-f(1)^2 \\bigr) \\cdot f(p^2) +\n",
    "                        \\bigl( f(p^2)-f(p)^2 \\bigr) \\cdot f(p) +\n",
    "                        \\bigl( f(p^4) - f(p^2)^2 \\bigr) \\cdot f(1) \\\\\n",
    "= \\; & 0 \\cdot f(p^2) + f(p^2) \\cdot f(p) - f(p)^2 \\cdot f(p) + f(p^4) - f(p^2)^2 \\\\\n",
    "= \\; & f(p^2) \\cdot f(p) - f(p)^3 + f(p^4) - f(p^2)^2 \n",
    "\\end{align}$\n",
    "\n",
    "\n",
    "This is not an obvious solution... let's use Theorem 2.8. This is recursive so we begin with $n=1$, \n",
    "then get the inverse at $n=p$, then finally at $n=p^2$.\n",
    "\n",
    "\n",
    "$\\begin{align}\n",
    "& f^{-1}(1) = 1/f(1) = 1 \n",
    "\\end{align}$\n",
    "\n",
    "\n",
    "The sum over divisors for $n=p$ is just one term with $d=1$.\n",
    "\n",
    "\n",
    "$\\begin{align}\n",
    "& f^{-1}(p) =  -f(p)\n",
    "\\end{align}$\n",
    "\n",
    "\n",
    "The sum over divisors for $n=p^2$ is two terms with $d = 1$ and $d = p$.\n",
    "\n",
    "\n",
    "$\\begin{align}\n",
    "& f^{-1}(p^2) = -\\sum_{d|p^2 \\atop d<p^2} f(p^2/d) f^{-1}(d) = -\\sum_{d \\in \\{1, p\\}} f(p^2/d) f^{-1}(d)\n",
    "\\end{align}$\n",
    "\n",
    "\n",
    "$\\begin{align}\n",
    "& f^{-1}(p^2) = -f(p^2) - f(p) \\cdot (-f(p)) = f(p)^2 - f(p^2)\n",
    "\\end{align}$\n",
    "\n",
    "\n",
    "&#x2610; \n",
    "\n",
    "\n",
    "\n",
    "### 2.26 For $f$ multiplicative: Show $f$ is *completely* multiplicative if and only if $f^{-1}(p^a)=0$ for all primes $p$ and all integers $a \\ge 2$.\n",
    "\n",
    "\n",
    "For this 'if and only if' proof we show $A \\implies B$ and $B \\implies A$. \n",
    "\n",
    "\n",
    "I write the Dirichlet inverse of $f$ as $g$. \n",
    "\n",
    "\n",
    "Suppose $f$ is *completely multiplicative*. Then from Thm 2.17 $g = \\mu f$.\n",
    "The $\\mu$ factor means that for argument $n$ squareful the inverse function\n",
    "$g(n) = 0$. So in the forward direction: If $f$ is $CX$ then the D-inverse $g$ \n",
    "is $0$ for all primes $p$ raised to the power $a \\ge 2$. \n",
    "\n",
    "\n",
    "Suppose $f$ is $X$ with D-inverse $g$, where for any prime $p$ and $a \\ge 2$ we have $g(p^a) = 0$. \n",
    "\n",
    "Then $g(p^2) = 0$. From problem 2.25: For $f$ multiplicative: \n",
    "$g(p^2) = f(p)^2 - f(p^2)$. Therefore $f(p)^2 = f(p^2)$. Now (following Chip) we use the \n",
    "recursion formula below to find more generally that $f(p^a) = f(p)^a$ where $a \\ge 2$ and \n",
    "by Thm 2.13b this implies $f$ is completely multiplicative.\n",
    "\n",
    "From Thm 2.8 let us calculate $g(p)$ and then more generally $g(p^{a \\ge 2})$ (which is of course zero):\n",
    "\n",
    "\n",
    "$\\begin{align}\n",
    "g(p) = \\; -f(p)\n",
    "\\end{align}$\n",
    "\n",
    "\n",
    "This is the Thm 2.8 recursion sum with $n=p$ reduced to one term ($d = 1$) by the condition $d < p$. Now for $a \\ge 2$:\n",
    "\n",
    "\n",
    "$\\begin{align}\n",
    "g(p^a) \n",
    "= \\; & - \\sum_{d|p^a \\atop d < p^a} f(p^a/d) \\cdot g(d) \\\\\n",
    "= \\; & - \\sum_{i=0}^{a-1} f(p^{a-i}) \\cdot g(p^i) \\\\\n",
    "\\end{align}$\n",
    "\n",
    "\n",
    "As this sum entails $g(p^i)$ it reduces to just two terms since $g(p^{a>1})=0$.\n",
    "\n",
    "\n",
    "$\\begin{align}\n",
    "g(p^a) \n",
    "= \\; & 0 \\\\\n",
    "= \\; & -f(p^a) \\cdot 1 - f(p^{a-1}) \\cdot g(p) \\\\\n",
    "= \\; & -f(p^a) - f(p^{a-1}) \\cdot (-f(p)) \\\\\n",
    "\\end{align}$\n",
    "\n",
    "\n",
    "Solving for $f(p^a)$:\n",
    "\n",
    "\n",
    "$\\begin{align}\n",
    "f(p^a) = f(p^{a-1}) \\cdot f(p)\n",
    "\\end{align}$\n",
    "\n",
    "\n",
    "This is not the same as $f(p^a) = f(p)^a$ but we can get to that by induction starting with\n",
    "(established above) $f(p^2) = f(p)^s$:\n",
    "\n",
    "\n",
    "$\\begin{align}\n",
    "& f(p^3) = f(p^2) \\cdot f(p) = f(p)^2 \\cdot f(p) = f(p)^3 \\\\\n",
    "& f(p^4) = f(p^3) \\cdot f(p) = f(p)^3 \\cdot f(p) = f(p)^4 \\\\\n",
    "& f(p^5) = f(p^4) \\cdot f(p) = f(p)^4 \\cdot f(p) = f(p)^5 \\\\\n",
    "& \\cdots\n",
    "\\end{align}$\n",
    "\n",
    "So to summarize: It was fast to show that $f$ completely multiplicative results in an inverse\n",
    "that includes $\\mu$ which produces zero when fed a squareful argument; including $p^a$. That\n",
    "is the $A \\implies B$ part of the proof. \n",
    "\n",
    "\n",
    "In the other direction, but with $f$ multiplicative established: The result from the previous\n",
    "problem can be used as a induction proof starting point -- working out the recursion formula\n",
    "for the inverse $g$ that yields $f(p^a) = f(p)^a$ for $a \\ge 2$. This rationale depends on\n",
    "the condition that $g(p^a) = 0$. From this result Thm 13.b states that $f$ is *completely*\n",
    "multiplicative. Consequently -- reverting to index notation $g = f^{-1}$:\n",
    "\n",
    "\n",
    "$f \\; X$ is in fact $CX \\iff f^{-1}(p^{a \\ge 2}) = 0. \\;\\;$ &#x2610; \n",
    "\n",
    "\n",
    "### 2.27 (a) and (b)\n",
    "\n",
    "#### 2.27 (a) For $f$ completely multiplicative, show $f \\cdot (g*h) = (f \\cdot g) * (f \\cdot h)$ for all arithmetic functions $g$ and $h$.\n",
    "\n",
    "\n",
    "\n",
    "$\\begin{align}\n",
    "f(g*h) = \\; & f \\cdot \\sum_{d|n} g(d) \\cdot h(n/d)\\\\\n",
    "= \\; & \\sum_{d|n} f(d)g(d) \\cdot f(n/d)h(n/d) \\\\\n",
    "= \\; & fg * fh\n",
    "\\end{align}$\n",
    "\n",
    "\n",
    "&#x2610; \n",
    "\n",
    "#### 2.27 (b) If $f$ is multiplicative and if the relation in (a) above holds for $g=\\mu$ and $h=\\mu^{-1}$, prove that $f$ is completely multiplicative.\n",
    "\n",
    "\n",
    "We have $f \\; X$ and $f \\cdot (\\mu * u) = f \\cdot I = f \\mu * f u$.\n",
    "\n",
    "\n",
    "Taking $n = 1, 2, 3, \\dots$ we see $f \\cdot I = I$. \n",
    "\n",
    "\n",
    "We see as well that $(f\\cdot u)(n) = f(n) \\cdot 1 = f(n)$.\n",
    "\n",
    "\n",
    "Therefore $(f \\cdot \\mu) * f = I$ and so $f^{-1} = f \\cdot \\mu$. By Theorem 2.17 $f$ is completely multiplicative. &#x2610;\n",
    "\n",
    "#### 2.28 Multiplicative function proof\n",
    "\n",
    "\n",
    "##### 2.28(a) \n",
    "\n",
    "\n",
    "If $f(n)$ is *completely multiplicative* prove for any arithmetic\n",
    "function $g(n)$ where $g(1) \\ne 0$: That ${(f \\cdot g)}^{-1} = f \\cdot {g}^{-1}$.\n",
    "\n",
    "\n",
    "Recalling that $f \\cdot g (n) = f(n) \\cdot g(n)$ it helps to view the composite\n",
    "function $f \\cdot g$ for a moment as \"some function $a(n)$\". From this step: The\n",
    "*to be proven* of the problem concerns the inverse of $a(n)$, in fact a \n",
    "*Dirichlet* inverse. So the notation of this problem includes two forms of \n",
    "multiplication: Dirichlet convolution and the implicit multiplication of \n",
    "composite functions: $a = f \\cdot g = f(n) \\cdot g(n)$. \n",
    "\n",
    "\n",
    "This distinction of types of multiplication comes up in problem 17 and is \n",
    "also mentioned at the top in the *ground rules*.\n",
    "\n",
    "\n",
    "Now on to the nuts and bolts. \n",
    "\n",
    "\n",
    "Let's take the obvious step of forming the Dirichlet product of $f \\cdot g$ with \n",
    "$f \\cdot {g}^{-1}$. Note that ${g}^{-1}$ exists and is unique because of that\n",
    "condition $g(1) \\ne 0$. \n",
    "\n",
    "$\\begin{align}\n",
    "(f \\cdot g) * (f \\cdot {g}^{-1}){|}_{n}\n",
    "= \\; & \\sum_{d|n} f(d) \\cdot g(d) \\cdot f(\\frac{n}{d}) \\cdot {g}^{-1}(\\frac{n}{d}) \\\\\n",
    "= \\; & f(n) \\cdot \\sum_{d|n} g(d) \\cdot {g}^{-1}(\\frac{n}{d}) \\\\\n",
    "= \\; & f(n) \\cdot (g * {g}^{-1}) \\\\\n",
    "= \\; & f(n) \\cdot I(n) \\\\\n",
    "= \\; & I(n) \\\\\n",
    "\\end{align}$\n",
    "\n",
    "\n",
    "The last step above uses the fact that a completely multiplicative function $f$\n",
    "must have $f(1) = 1$ so for all positive $n$ the composite function $f \\cdot I$\n",
    "will have values $\\{ 1, 0, 0, 0, \\dots \\}$. \n",
    "\n",
    "\n",
    "As the inverse of $g$ exists and is unique; and as we see $f \\cdot {g}^{-1}$\n",
    "meets the criterion of an inverse we are done. $\\;\\;$&#x2610;\n",
    "\n",
    "\n",
    "\n",
    "##### 28(b) \n",
    "\n",
    "Suppose now that $f$ is multiplicative\n",
    "and set $g = {\\mu}^{-1}$. Establish that $f$ is completely multiplicative\n",
    "if (as in part (a)) we have ${(f \\cdot g)}^{-1} = f \\cdot {g}^{-1}$.\n",
    "\n",
    "\n",
    "This will use Thm 2.17: Suppose $f$ is multiplicative: Then $f$ is *completely*\n",
    "multiplicative if and only if ${f}^{-1} = \\mu \\cdot f \\; \\; \\forall \\; \\; n \\ge 1$.\n",
    "\n",
    "Now translate ${(f \\cdot g)}^{-1} = f \\cdot {g}^{-1}$, where \n",
    "$g = {\\mu}^{-1} = u$: \n",
    "\n",
    "$\\begin{align}{(f \\cdot u)}^{-1} = f \\cdot \\mu \\end{align}$.\n",
    "\n",
    "As $u(n) = 1$ we have $(f \\cdot u) = f$ and so \n",
    "${f}^{-1} = f \\cdot \\mu$ per 2.17 so $f$ is $CX.\\;\\;$&#x2610;\n",
    "\n",
    "### 2.29 Two part problem on a multiplicative identity\n",
    "\n",
    "\n",
    "#### 2.29 First part: Prove that for every arithmetical function $f$ there is a multiplicative arithmetical function $g$ such that the expression below holds:\n",
    "\n",
    "\n",
    "$\\begin{align}\\sum_{k=1}^{n} f \\big( (k, n) \\big) = f * g \\end{align}$\n",
    "\n",
    "\n",
    "Does Tommy mean 'one size fits all', i.e. there is a single $g$ that will suffice for any and all\n",
    "$f$? Or is it that $g$ exists and varies with $f$? \n",
    "\n",
    "\n",
    "As $(k, n)$ being the *gcd* of $k$ and $n$ will always be a divisor of $n$: We\n",
    "can anticipate this is already looking like some sort of Dirichlet convolution.\n",
    "Let's follow the trail...\n",
    "\n",
    "\n",
    "$\\begin{align}\n",
    "\\sum_{k=1}^{n} f \\big( (k, n) \\big) \n",
    "= \\; & f((1, n )) + f((2, n)) + f((3, n)) \\dots + f((n, n)) \\\\\n",
    "= \\; & \\sum_{d|n} f(d) \\cdot \\sum_{{k \\in \\{1, \\dots, n\\} } \\atop {\\ni (k, n) = d}} 1\n",
    "\\end{align}$\n",
    "\n",
    "\n",
    "That second sum-of-ones on the RHS could use some English. The rationale\n",
    "is that the original sum using $k$ from $1$ to $n$ will produce only divisors\n",
    "of $n$ in the argument of $f()$. This will hit *all* divisors of $n$ at least \n",
    "once including both $1$ and $n$. So this motivates the sum over $d|n$ summing\n",
    "$f(d)$ scaled by the number of occurrences of that divisor $d$ from that \n",
    "$1$ to $n$ \"$k$-scan\".\n",
    "\n",
    "\n",
    "Now that second sum in the lower righthand side is: Just the count of \n",
    "those occurrences for a given $d$. It is a $+1$ for \"only the values of \n",
    "$k$ that produce a given divisor $d$\". \n",
    "\n",
    "\n",
    "\n",
    "From the Proof of Thm 2.2 the right sum is $\\varphi(\\frac{n}{d})$ so\n",
    "we get $\\sum_{k=1}^{n} f \\big( (k, n) \\big) = f * \\varphi \\big|_{n}). \\;\\;\\;$&#x2610;\n",
    "\n",
    "\n",
    "It would appear Tommy had the totient in mind as a single function that\n",
    "will serve for any and all $f$.\n",
    "\n",
    "### 2.29 Second part: Use the identity from the first part to prove:\n",
    "\n",
    "\n",
    "$\\begin{align}\n",
    "\\sum_{k=1}^{n} (k, n) \\mu\\big( (k, n) \\big) = \\mu(n)\n",
    "\\end{align}$\n",
    "\n",
    "\n",
    "Here the function $f$ from the first part is specifically the \n",
    "composite function $n \\cdot \\mu(n)$, more formally $(N \\cdot \\mu)(n)$. \n",
    "Applying the identity from the first part: \n",
    "\n",
    "$\\begin{align}\n",
    "\\sum_{k=1}^{n} (N \\cdot \\mu)((k, n)) = (N \\cdot \\mu) * \\varphi\n",
    "\\end{align}$\n",
    "\n",
    "\n",
    "As $N(n)$ is completely multiplicative, by Theorem 2.17 we have $N \\cdot \\mu = \\mu \\cdot N = N^{-1}$.\n",
    "Also Theorem 2.3 states that $\\varphi = \\mu * N$. We now have: \n",
    "\n",
    "\n",
    "$\\begin{align}\n",
    "\\sum_{k=1}^{n} (N \\cdot \\mu)((k, n)) = N^{-1} * \\varphi = N^{-1} * N * \\mu = \\mu.\n",
    "\\end{align}\\;\\;\\;\\;\\;$&#x2610; \n",
    "\n",
    "\n",
    "\n",
    "### 2.30 Bell series if and only if proof\n",
    "\n",
    "\n",
    "I paraphrase the statement of the problem a bit:\n",
    "\n",
    "\n",
    "Let $f$ be multiplicative and $g$ be an arithmetic function. Suppose\n",
    "for all primes $p$ and all $n \\ge 1$ that \n",
    "\n",
    "$\\begin{align}\n",
    "f(p^{n+1}) = f(p) f(p^n) - g(p)f(p^{n-1})\n",
    "\\end{align}$\n",
    "\n",
    "\n",
    "Show this is true if and only if the Bell series for $f$ has the form\n",
    "\n",
    "\n",
    "$\\begin{align}\n",
    "f_p(x) = \\frac{1}{1 - f(p) x + g(p) x^2}\n",
    "\\end{align}$\n",
    "\n",
    "\n",
    "The obvious idea to try is to write the definition of the Bell series \n",
    "(an infinite polynomial) in terms of an arbitrary prime $p$ and the free \n",
    "variable $x$. Following Chip directly I will do so and then proceed along\n",
    "an 'if and only if' sequence of steps. I think the idea is to produce a logical \n",
    "sequence justifiable in both forward and reverse directions to achieve\n",
    "the desired if-and-only-if-ness $\\iff$. \n",
    "\n",
    "$\\begin{align}\n",
    "f_{p}(x) = \\; & \\sum_{n=0}^{\\infty} f(p^{n}) x^n \\\\\n",
    "= \\; & 1 + f(p)x + \\sum_{n=2}^{\\infty} f(p^{n}) x^n \\\\\n",
    "= \\; & 1 + f(p)x + \\sum_{n=2}^{\\infty} \\bigl( f(p)f(p^{n-1}) - g(p)f(p^{n-2})\\bigr) x^n \\textrm{ using the supposition}\\\\\n",
    "\\end{align}$\n",
    "\n",
    "By inspection: Changing the sum index to begin at $2$ retains the argument as a valid expression.\n",
    "\n",
    "\n",
    "Now the steps are to break the infinite sum into its two constituents and shift the respective\n",
    "starting indices to arrive at a tractable equality.\n",
    "\n",
    "$\\begin{align}\n",
    "f_{p}(x) = \\; & 1 + f(p) \\; x + \\sum_{n=2}^{\\infty} f(p)f(p^{n-1}) x^n - \\sum_{n=2}^{\\infty} g(p)f(p^{n-2}) x^n \\\\\n",
    "= \\; & 1 + f(p) \\; x + f(p) \\sum_{n=2}^{\\infty} f(p^{n-1}) x^n - g(p) \\sum_{n=2}^{\\infty} f(p^{n-2}) x^n \\textrm{ ...and now to shift indexing...}\\\\\n",
    "= \\; & 1 + f(p) \\; x + f(p) x \\sum_{n=1}^{\\infty} f(p^{n}) x^n - g(p) x^2 \\sum_{n=0}^{\\infty} f(p^{n}) x^n \\\\\n",
    "= \\; & 1 + f(p) \\; x \\; f_{p}(x) - g(p) \\; x^2 \\; f_{p}(x) \\\\\n",
    "\\end{align}$\n",
    "\n",
    "\n",
    "The final expression is linear in $f_{p}(x)$, easily resolved:\n",
    "\n",
    "$\\begin{align}\n",
    "f_p(x) = 1 + (f(p) \\; x) \\; f_{p}(x) - (g(p) \\; x^2) \\; f_{p}(x) \\\\\n",
    "\\end{align}$\n",
    "\n",
    "\n",
    "$\\begin{align}\n",
    "f_p(x) = \\frac{1}{1 - f(p) x + g(p) x^2}\\;\\;\\;\n",
    "\\end{align}$\n",
    "\n",
    "\n",
    "The if and only if argument I suppose stems from these algebraic steps all being reversible.\n",
    "$\\;\\;\\;$&#x2610; \n",
    "\n"
   ]
  },
  {
   "cell_type": "code",
   "execution_count": null,
   "id": "5290dfe5-6ad1-4ef5-94a2-78aac1f6ecf8",
   "metadata": {},
   "outputs": [],
   "source": []
  }
 ],
 "metadata": {
  "kernelspec": {
   "display_name": "Python 3 (ipykernel)",
   "language": "python",
   "name": "python3"
  },
  "language_info": {
   "codemirror_mode": {
    "name": "ipython",
    "version": 3
   },
   "file_extension": ".py",
   "mimetype": "text/x-python",
   "name": "python",
   "nbconvert_exporter": "python",
   "pygments_lexer": "ipython3",
   "version": "3.13.4"
  }
 },
 "nbformat": 4,
 "nbformat_minor": 5
}
