{
 "cells": [
  {
   "cell_type": "markdown",
   "id": "b5d187b0-7d3e-448a-8320-b302502087cc",
   "metadata": {},
   "source": [
    "### Problems 2.31 through 2.40 \n",
    "#### Includes the generalized Möbius function"
   ]
  },
  {
   "cell_type": "markdown",
   "id": "106aa66a-a450-490b-a5cb-c0668f4cff9f",
   "metadata": {},
   "source": [
    "### 2.31\n",
    "\n",
    "\n",
    "$\\begin{align}\n",
    "\\dots\n",
    "\\end{align}$\n",
    "\n",
    "\n",
    "### 2.32\n",
    "\n",
    "\n",
    "$\\begin{align}\n",
    "\\dots\n",
    "\\end{align}$\n",
    "\n",
    "\n",
    "### 2.33\n",
    "\n",
    "\n",
    "$\\begin{align}\n",
    "\\dots\n",
    "\\end{align}$\n",
    "\n",
    "\n",
    "### 2.34\n",
    "\n",
    "\n",
    "$\\begin{align}\n",
    "\\dots\n",
    "\\end{align}$\n",
    "\n",
    "### 2.35 Prove $h(n)$ as defined below is multiplicative\n",
    "\n",
    "\n",
    "Defining $h(n)$: Let $f$ and $g$ be multiplicative functions and $a$ and $b$ \n",
    "positive integers with $a \\ge b$.\n",
    "\n",
    "\n",
    "$\\begin{align}\n",
    "\\textrm{Define } h(n) = \\sum_{d^a|n} f \\Bigl( \\frac{n}{d^a} \\Bigr) \\; g \\Bigl( \\frac{n}{d^b} \\Bigr)\n",
    "\\end{align}$\n",
    "\n",
    "\n",
    "Here $d$ is a divisor of $n$ but the sum is constrained to only $a$th powers of $d$ that divide $n$.\n",
    "As $b$ is less than or equal to $a$: In such cases $n$ is divisible by $d^b$ as well.\n",
    "Take $n=24$: Then for $a=2$ the sum would be over $\\{1, 4\\}$ and for $a=3$ the sum would be over $\\{1, 8\\}$.\n",
    "\n",
    "The plan is obvious enough: Show that for $(m, n) = 1 \\textrm{ we have } h(m) \\cdot h(n) = h(m \\cdot n)$.\n",
    "This seems to be the downhil direction in Chip's solution. I also follow his notational point of departure:\n",
    "From $(m, n) = 1$ we can imagine divisors $c$ and $d$ of $m$ and $n$ respectively for which it will also be\n",
    "the case that $(m/c, n/d) = 1$. \n",
    "\n",
    "\n",
    "$\\begin{align}\n",
    "h(m) \\cdot h(n) = \n",
    "\\sum_{c^a|m} f \\bigl( \\frac{m}{c^a} \\bigr) g \\bigl( \\frac{m}{c^b} \\bigr) \\cdot \n",
    "\\sum_{d^a|n} f\\bigl( \\frac{n}{d^a} \\bigr) g \\bigl( \\frac{n}{d^b} \\bigr)\n",
    "\\end{align}$\n",
    "\n",
    "\n",
    "Multiplying these two sums produces a grand sum over all allowed pairs of $c^a$ and $d^a$; where with $(c, d) = 1$\n",
    "this is equivalent to indexing all possible composite pairs $e = c \\cdot d$.\n",
    "\n",
    "\n",
    "$\\begin{align}\n",
    "h(m) \\cdot h(n) = \\; &\n",
    "\\sum_{c^a|m \\atop d^a|n} f \\bigl( \\frac{m}{c^a} \\bigr) \\cdot g \\bigl( \\frac{m}{c^b} \\bigr) \\cdot \n",
    "f\\bigl( \\frac{n}{d^a} \\bigr) \\cdot g \\bigl( \\frac{n}{d^b} \\bigr) \\\\\n",
    "= \\; & \\sum_{c^a|m \\atop d^a|n} f \\bigl( \\frac{m \\cdot n}{(cd)^a} \\bigr) \\cdot g \\bigl( \\frac{m \\cdot n}{(cd)^b} \\bigr) \\\\\n",
    "= \\; & \\sum_{e^a|mn} f \\bigl( \\frac{m \\cdot n}{e^a} \\bigr) \\cdot g \\bigl( \\frac{m \\cdot n}{e^b} \\bigr) \\\\\n",
    "= \\; & h(m \\cdot n)\n",
    "\\end{align}$\n",
    "\n",
    "\n",
    "&#x2610;"
   ]
  },
  {
   "cell_type": "markdown",
   "id": "8285ca91-c4e0-49f1-84f4-1073494e78b2",
   "metadata": {},
   "source": [
    "### Introducing Möbius functions of order $k \\ge 1$\n",
    "\n",
    "\n",
    "Define $\\mu_k(n)$ by cases dependent on the factorization of $n$:\n",
    "\n",
    "\n",
    "- Case 1: $\\mu_k(1) = 1$\n",
    "- Case 2: $\\mu_k(n) = 0$ when any $p^{k+1}|n$\n",
    "- Case 3: $\\mu_k(n) = (-1)^r$ if $n= \\prod_{j=1}^r p_j^k \\cdot \\prod_{i} p_i^{a_i < k}$\n",
    "- Case 4: $\\mu_k(n) = 1$ otherwise\n",
    "\n",
    "\n",
    "Analogs to $\\mu(n)$: We have $\\mu_k(1)=\\mu(1)=1$. \n",
    "$\\mu(n)=0$ when $n$ has a square divisor; and $\\mu_k(n)=0$ when\n",
    "$n$ has a *power-$(k+1)$* divisor.\n",
    "When $n$ fails to achieve winning factors $p^k: \\; \\mu_{k}(n)$ behaves like $\\mu_k(1) = 1$."
   ]
  },
  {
   "cell_type": "markdown",
   "id": "965d0dec-5272-4d1b-b125-54cc51fea331",
   "metadata": {},
   "source": [
    "### 2.36 Show that for $k \\ge 1$ we have $\\mu_k(n^k) = \\mu(n)$\n",
    "\n",
    "\n",
    "With $k=1$ a trivial equivalence, we are concerned with $k > 1$; and the point of \n",
    "the problem is that the $n^k$ argument in an order-$k$ Möbius functions has\n",
    "a *constrained* prime factorization; so $\\mu_k(n^k)$ matches\n",
    "$\\mu(n)$. I show this equality condition 'is fine' by cases:\n",
    "\n",
    "\n",
    "\n",
    "Case 1: $n=1$ is fine as $\\mu_k(1^k) = \\mu(1) = 1$.\n",
    "\n",
    "\n",
    "Case 2: $n$ is not square free; $n$ has divisor $p^{q \\; \\ge \\; 2}$ so $\\mu(n)=0$. \n",
    "This is fine as $p^{(k \\cdot q) \\; \\gt \\; k} \\; \\big| \\; n^k$ so $\\mu_k(n^k) = 0$.\n",
    "\n",
    "\n",
    "Case 3: Suppose $n$ is square free: $n = \\prod_{i=1}^{r} p_i$. \n",
    "Then $n^k = \\prod_{i=1}^r p_i^k$ and $\\mu(n) = (-1)^r = \\mu_k(n^k)$.\n",
    "\n",
    "\n",
    "There are no other cases available so we are done.$\\;\\;$ &#x2610; \n",
    "\n",
    "\n",
    "Chip's more rigorous solution is an induction proof on $k$."
   ]
  },
  {
   "cell_type": "markdown",
   "id": "32a373be-1f01-4c68-8272-02e4c606859f",
   "metadata": {},
   "source": [
    "### 2.37 Show that $\\mu_k(n)$ is multiplicative.\n",
    "\n",
    "\n",
    "I proceed by cases on $\\mu_k(m \\cdot n)$ where $(m, n) = 1$. \n",
    "\n",
    "\n",
    "(Aside, $\\mu_k$ is not *completely* multiplicative by counterexample: $\\mu_3(27) = -1 \\ne \\mu_3(9) \\cdot \\mu_3(3)$.)\n",
    "\n",
    "\n",
    "Case 0: For $m = 1$ we have $\\mu_k(m \\cdot n) = 1 \\cdot \\mu_k(n)$. \n",
    "\n",
    "\n",
    "For both $m, n > 0$: \n",
    "\n",
    "Case 1: $p^{(a>k)} \\; | \\; m \\implies \\mu_k(m \\cdot n) = 0.$\n",
    "\n",
    "Case 2: There is no prime $p$ such that $p^k \\; | \\; m \\; \\textrm{ or } \\; n$. \n",
    "In this case $\\mu_k(m \\cdot n) = 1 = \\mu_k(m) \\cdot \\mu_k(n)$.\n",
    "\n",
    "Case 3: $k$-powers of prime factors are present in amounts $q$ and $r$ for $m$ and $n$ respectively.\n",
    "Then $\\mu_k(m \\cdot n) = (-1)^{q + r} = \\mu_k(m) \\cdot \\mu_k(n)\\;\\;\\;\\;\\;\\;\\;$ &#x2610;"
   ]
  },
  {
   "cell_type": "markdown",
   "id": "51b3be0b-2d8c-4fcf-9b8b-10be198fee9e",
   "metadata": {},
   "source": [
    "### 2.38  Show that if $k \\ge 2$ then \n",
    "\n",
    "\n",
    "$\\begin{align}\n",
    "\\mu_k(n) = \\sum_{d^k|n} \\mu_{k-1}\\Bigl( \\frac{n}{d^k} \\Bigr) \\mu_{k-1}\\Bigl( \\frac{n}{d} \\Bigr)\n",
    "\\end{align}$\n",
    "\n",
    "\n",
    "Both sides are multiplicative (see problems 2.37 and 2.35 for this result, lhs and rhs respectively).\n",
    "The rhs could probably use a little more checking. But to continue: With multiplicative functions it\n",
    "will suffice to show the desired result for argument $p^a$. \n",
    "\n",
    "\n",
    "The case of $a=0$ so $n=1$ checks out: Both sides are $1$.\n",
    "\n",
    "\n",
    "For the case where $n = p^{k+1}$: The lhs evaluates to $0$. \n",
    "In the rhs sum: We have two terms to consider, $d=1$ and $d=p$ with the \n",
    "righthand $\\mu_{k-1}$ having corresponding arguments $p^{k+1}$ and \n",
    "$p^k$. These both evaluate as $0$, case closed.\n",
    "\n",
    "\n",
    "This leaves two remaining cases: $n = p^k$ and $n = p^{j < k}$. For both: The lhs $= 1$.\n",
    "\n",
    "For $n = p^k$ the rhs is two nonzero terms: $d=1$ and $d=p$. \n",
    "This gives $1 \\cdot 0 + (-1) \\cdot \\mu_{k-1}(p^{k-1}) = -1 \\cdot -1 = 1$, correct. \n",
    "\n",
    "For $n = p^j$ the rhs is one terms, $d = 1$. This evaluates as $1 \\cdot 1 = 1$, correct. &#x2610;"
   ]
  },
  {
   "cell_type": "markdown",
   "id": "3a43ffee-200c-45b6-93f3-1707304a01d6",
   "metadata": {},
   "source": [
    "### 2.39 Show that if $k \\ge 1$ then $\\bigl| \\mu_k(n) \\bigr| = \\sum_{d^{k+1}|n}\\mu(d)$\n",
    "\n",
    "Problem 2.6 proves (slightly paraphrased):\n",
    "\n",
    "\n",
    "$\\begin{align}\n",
    "\\sum_{d^{k+1}|n} \\mu(d) = \\begin{cases}\n",
    "0 & \\textrm{ if } m^{k+1}|n \\textrm{ for some } m > 1 \\\\\n",
    "1 & \\textrm{ otherwise }\n",
    "\\end{cases}\n",
    "\\end{align}$\n",
    "\n",
    "$\\begin{align}\n",
    "\\mu(n) = \\begin{cases} \n",
    "1 & \\textrm{ if } n = 1 \\\\\n",
    "-1^k & \\textrm{ if } n \\textrm{ is the product of } k \\textrm{ distinct primes } \\\\\n",
    "0 & \\textrm{ otherwise }\n",
    "\\end{cases}\n",
    "\\end{align}$\n",
    "\n",
    "\n",
    "Let's check the four cases for argument $n$:\n",
    "\n",
    "\n",
    "- Case 1 $\\;\\;n = 1$ so $|\\mu_{k}(1)| = 1$, confirmed, done.\n",
    "- Case 2 $\\;\\;n$ has a factor $p^{k+1}$ so $|\\mu_{k}(n)| = 0$, RHS is likewise $0$ from the problem 2.6 result, done.\n",
    "- Case 3 $\\;\\;n$ has $r$ factors of the form $p^k$ but no higher exponents: $|\\mu_{k}(n)| = 1$, RHS has only $d=1$, confirmed, done.\n",
    "- Case 4 $\\;\\;n$ has only factors $p^{j < k}$: $|\\mu_{k}(n)| = 1$, RHS has only $d=1$, confirmed, done.\n",
    "\n",
    "\n",
    "&#x2610;"
   ]
  },
  {
   "cell_type": "markdown",
   "id": "35dfa7f1-87ed-4165-85ef-b117a59f7af1",
   "metadata": {},
   "source": [
    "### 2.40 Show that for each prime $p$ the Bell series for $u_k$ is given by \n",
    "\n",
    "\n",
    "$\\begin{align}(\\mu_k)_p(x) = \\frac{1-2x^k+x^{k+1}}{1-x}\\end{align}$\n",
    "\n",
    "\n",
    "This is interesting as the choice of prime $p$ evaporates from the end result.\n",
    "\n",
    "\n",
    "The Bell series of $\\mu_k \\textrm{ mod } p$ is defined in this case\n",
    "\n",
    "\n",
    "$\\begin{align}(\\mu_k)_p(x) = \\sum_{n=0}^{\\infty} \\mu_k(p^n)x^n\\end{align}$\n",
    "\n",
    "\n",
    "What follows is valid for $k=1$ but is written more in the spirit of $k>1$. \n",
    "The argument of the infinite sum becomes zero when $n$ exceeds $k$\n",
    "so the sum can be truncated at $k$; and then rewritten in a more concrete form: \n",
    "\n",
    "\n",
    "$\\begin{align}(\\mu_k)_p(x) = \\sum_{n=0}^{k} \\mu_k(p^n)x^n = 1 + x + \\sum_{n=2}^{k} \\mu_k(p^n)x^n\\end{align}$\n",
    "\n",
    "\n",
    "The prime $p$ is raised to a value less than $k$ for most of this sum, i.e. $\\mu_k = 1$;\n",
    "and the final term $n=k$ resolves to $(-1)^1$:\n",
    "\n",
    "\n",
    "$\\begin{align}(\\mu_k)_p(x) = \\sum_{n=0}^{k} \\mu_k(p^n)x^n = 1 + x + \\sum_{n=2}^{k-1} x^n - x^k\\end{align}$\n",
    "\n",
    "\n",
    "Observing the pattern:\n",
    "\n",
    "\n",
    "$\\begin{align}k=1: (\\mu_k)_p(x) = 1-x\\end{align}$\n",
    "\n",
    "\n",
    "$\\begin{align}k=2: (\\mu_k)_p(x) = 1 + x - x^2\\end{align}$\n",
    "\n",
    "\n",
    "$\\begin{align}k=3: (\\mu_k)_p(x) = 1 + x + x^2 - x^3\\end{align}$\n",
    "\n",
    "\n",
    "$\\begin{align}k=4: (\\mu_k)_p(x) = 1 + x + x^2 + x^3 - x^4\\end{align}$\n",
    "\n",
    "\n",
    "$\\begin{align}k:(\\mu_k)_p(x) = 1 + x + x^2 + \\dots + x^{k-1} - x^k\\end{align}$\n",
    "\n",
    "\n",
    "In the spirit of a telescoping series: Multiply the last (general) expression above by $1-x$: \n",
    "\n",
    "\n",
    "$\\begin{align}(1-x) \\cdot (1 + x + x^2 + \\dots + x^{k-1} - x^k) =  \n",
    "1 + x + x^2 + \\dots + x^{k-1} - x^k - x - x^2 - x^3 - \\dots - x^{k-1} - x^{k} + x^{k+1} = 1 - 2x^k + x^{k+1}\\end{align}$\n",
    "\n",
    "\n",
    "So the general expression can be written \n",
    "\n",
    "\n",
    "$\\begin{align}1 + x + x^2 + \\dots + x^{k-1} - x^k = \\frac{1 - 2x^k + x^{k+1}}{1-x} = (\\mu_k)_p(x).\\;\\;\\end{align}$ &#x2610;"
   ]
  },
  {
   "cell_type": "code",
   "execution_count": null,
   "id": "3b58b917-2e82-4dda-b41c-f31e5c44d2a7",
   "metadata": {},
   "outputs": [],
   "source": []
  }
 ],
 "metadata": {
  "kernelspec": {
   "display_name": "Python 3 (ipykernel)",
   "language": "python",
   "name": "python3"
  },
  "language_info": {
   "codemirror_mode": {
    "name": "ipython",
    "version": 3
   },
   "file_extension": ".py",
   "mimetype": "text/x-python",
   "name": "python",
   "nbconvert_exporter": "python",
   "pygments_lexer": "ipython3",
   "version": "3.13.4"
  }
 },
 "nbformat": 4,
 "nbformat_minor": 5
}
